VST-introduction/verif_second_list_from_append_v2.v
@@ -112,7 +112,6 @@ Qed.
 (************************)
 (************************)
 
-
 (** Spec *)
 
 Definition add_spec := (** uses listrep*)
@@ -168,19 +167,6 @@ Definition add_void_spec' := (** uses listrep_cons*)
       RETURN (if eq_dec q nullval then nullval else n) (* returns 0 when there is no tail, and head otherwise, so n *)
       SEP (data_at sh (t_node) q n;  listrep sh il q).
 
-
-Definition free_spec := (** uses listrep_cons*)
-   DECLARE _free
-   WITH sh : share, p: val, q: val, il: list val, n:val
-   PRE [ tptr tvoid , tptr t_node]
-      PROP(writable_share sh) (* not sure this is ok to say *)
-      PARAMS (n; q) GLOBALS()
-      SEP (data_at sh (t_node) nullval n; listrep sh il q)
-   POST [ tvoid ]
-      PROP()
-      RETURN () (* no return value *)
-      SEP (data_at sh (t_node) q n;  listrep sh il q).
-
 Definition remove_spec := (* assume the list isn't empty *)
   DECLARE _remove
    WITH sh : share, q: val, il: list val, n:val            
@@ -195,16 +181,41 @@ Definition remove_spec := (* assume the list isn't empty *)
       SEP (data_at sh (t_node) q n; listrep sh il q). (* I did not free the node.. *)
 
 Definition remove_only_if_lst_spec := (* assume the list isn't empty *)
- DECLARE _remove
+ DECLARE _remove_only_if_lst
    WITH sh : share, q: val, il: list val, n:val            
    PRE [ tptr t_node]
       PROP(writable_share sh) (* not sure this is ok to say *)
       PARAMS (n) GLOBALS()
-      SEP (data_at sh (t_node) q n; listrep sh il q)
+      SEP (data_at sh (t_node) q n; listrep sh il q) (* q can be nullval meaning that there is only one node *)
    POST [ tvoid ]
       PROP()
       RETURN ()
-      SEP (data_at sh (t_node) q n; listrep sh il q). (* I did not free the node.. *)
+      SEP (data_at sh (t_node) q n; listrep sh il q). (* the node still exists *)
+
+Definition free_spec := (** uses listrep_cons*)
+ DECLARE _free
+   WITH sh : share, p: val, q: val, il: list val, n:val
+   PRE [ tptr tvoid , tptr t_node]
+      PROP(writable_share sh) (* not sure this is ok to say *)
+      PARAMS (n; q) GLOBALS()
+      SEP (data_at sh (t_node) nullval n; listrep sh il q)
+   POST [ tvoid ]
+      PROP()
+      RETURN () (* no return value *)
+      SEP (data_at sh (t_node) q n;  listrep sh il q).
+
+Definition alloc_spec := (* assume the list isn't empty *)
+ DECLARE _alloc
+   WITH sh : share, q: val, il: list val, n:val            
+   PRE [ tptr t_node]
+      PROP(writable_share sh)
+      PARAMS (n) GLOBALS()
+      SEP (data_at sh (t_node) q n; listrep sh il q) (* q can be nullval meaning that there is only one node *)
+   POST [ tptr tvoid ]
+      PROP()
+      RETURN (n) (* we return the head like in the pop function*)
+      SEP (data_at sh (t_node) q n; listrep sh il q). 
+
 
 
 (*Definition add_kmem_spec :=
@@ -220,7 +231,7 @@ DECLARE _add
       RETURN (r)
       SEP (listrep sh (s1++s2) r).
 *)
-Definition Gprog := [add_spec; add_spec'; add_void_spec; add_void_spec'; free_spec; remove_spec; remove_only_if_lst_spec].
+Definition Gprog := [add_spec; add_spec'; add_void_spec; add_void_spec'; free_spec; remove_spec; remove_only_if_lst_spec; alloc_spec].
 (*Definition Gprog := [add_spec; add_void_spec; remove_spec].*)
 
 (*Definition lseg (sh: share) (contents: list val) (x z: val) : mpred :=
@@ -308,6 +319,18 @@ forward_if.
 - forward. entailer!.
 Qed.
 
+Lemma body_alloc: semax_body Vprog Gprog f_alloc alloc_spec.
+Proof.
+start_function.
+forward. 
+forward_if (PROP () LOCAL (temp _lst (if eq_dec n nullval then nullval else q);
+                            temp _head n)
+                 SEP (data_at sh t_node q n; listrep sh il q)).
+
+- forward. entailer!. destruct (eq_dec n nullval); auto. subst. inversion H.
+- forward. entailer!.
+- forward.
+Qed.
 
 
 
